<?xml version="1.0"?>
<rdf:RDF xmlns="http://www.hsu-ifa.de/ontologies/VDI3682#"
     xml:base="http://www.hsu-ifa.de/ontologies/VDI3682"
     xmlns:obda="https://w3id.org/obda/vocabulary#"
     xmlns:rdf="http://www.w3.org/1999/02/22-rdf-syntax-ns#"
     xmlns:owl="http://www.w3.org/2002/07/owl#"
     xmlns:xml="http://www.w3.org/XML/1998/namespace"
     xmlns:VDI3682="http://www.hsu-ifa.de/ontologies/VDI3682#"
     xmlns:swrlb="http://www.w3.org/2003/11/swrlb#"
     xmlns:swrl="http://www.w3.org/2003/11/swrl#"
     xmlns:xsd="http://www.w3.org/2001/XMLSchema#"
     xmlns:rdfs="http://www.w3.org/2000/01/rdf-schema#"
     xmlns:swrla="http://swrl.stanford.edu/ontologies/3.3/swrla.owl#">
    <owl:Ontology rdf:about="http://www.hsu-ifa.de/ontologies/VDI3682">
        <owl:versionInfo>1.1.0</owl:versionInfo>
    </owl:Ontology>
    


    <!-- 
    ///////////////////////////////////////////////////////////////////////////////////////
    //
    // Annotation properties
    //
    ///////////////////////////////////////////////////////////////////////////////////////
     -->

    


    <!-- http://swrl.stanford.edu/ontologies/3.3/swrla.owl#isRuleEnabled -->

    <owl:AnnotationProperty rdf:about="http://swrl.stanford.edu/ontologies/3.3/swrla.owl#isRuleEnabled"/>
    


    <!-- 
    ///////////////////////////////////////////////////////////////////////////////////////
    //
    // Object Properties
    //
    ///////////////////////////////////////////////////////////////////////////////////////
     -->

    


    <!-- http://www.hsu-ifa.de/ontologies/VDI3682#ProcessOperatorIsAssignedToTechnicalResource -->

    <owl:ObjectProperty rdf:about="http://www.hsu-ifa.de/ontologies/VDI3682#ProcessOperatorIsAssignedToTechnicalResource">
        <owl:inverseOf rdf:resource="http://www.hsu-ifa.de/ontologies/VDI3682#TechnicalResourceIsAssignedToProcessOperator"/>
        <rdfs:domain rdf:resource="http://www.hsu-ifa.de/ontologies/VDI3682#Process"/>
        <rdfs:range rdf:resource="http://www.hsu-ifa.de/ontologies/VDI3682#TechnicalResource"/>
        <rdfs:comment>ObjectProperty that is used to indicate that a process operator is performed by a technical resource.</rdfs:comment>
    </owl:ObjectProperty>
    


    <!-- http://www.hsu-ifa.de/ontologies/VDI3682#TechnicalResourceIsAssignedToProcessOperator -->

    <owl:ObjectProperty rdf:about="http://www.hsu-ifa.de/ontologies/VDI3682#TechnicalResourceIsAssignedToProcessOperator">
        <rdfs:domain rdf:resource="http://www.hsu-ifa.de/ontologies/VDI3682#TechnicalResource"/>
        <rdfs:range rdf:resource="http://www.hsu-ifa.de/ontologies/VDI3682#Process"/>
        <rdfs:comment>ObjectProperty that is used to indicate that a process operator is performed by a technical resource.</rdfs:comment>
    </owl:ObjectProperty>
    


    <!-- http://www.hsu-ifa.de/ontologies/VDI3682#dependency -->

    <owl:ObjectProperty rdf:about="http://www.hsu-ifa.de/ontologies/VDI3682#dependency">
        <rdfs:domain>
            <owl:Class>
                <owl:unionOf rdf:parseType="Collection">
                    <rdf:Description rdf:about="http://www.hsu-ifa.de/ontologies/VDI3682#Energy"/>
                    <rdf:Description rdf:about="http://www.hsu-ifa.de/ontologies/VDI3682#Information"/>
                    <rdf:Description rdf:about="http://www.hsu-ifa.de/ontologies/VDI3682#Product"/>
                </owl:unionOf>
            </owl:Class>
        </rdfs:domain>
        <rdfs:range>
            <owl:Class>
                <owl:unionOf rdf:parseType="Collection">
                    <rdf:Description rdf:about="http://www.hsu-ifa.de/ontologies/VDI3682#Energy"/>
                    <rdf:Description rdf:about="http://www.hsu-ifa.de/ontologies/VDI3682#Information"/>
                    <rdf:Description rdf:about="http://www.hsu-ifa.de/ontologies/VDI3682#Product"/>
                </owl:unionOf>
            </owl:Class>
        </rdfs:range>
        <rdfs:comment>This ObjectProperty is not explicitly contained within the VDI 3682. It is used to describe dependencies of In- and Outputs. Due to open world assumption (OWA) the case that more than one In- or Outputs occur does always mean an alternative Input. For the case, that In- and Outputs are depending on each other, the ObjectProperty Dependency can be used. It can be interpreted as an &quot;AND&quot; constructor between In- and/or Outputs of a process.

E.g.: A process has two Inputs. If they are alternatives, then this fact must not  be explcitly modelled. If both Inputs have to go into the process, then the &quot;Dependency&quot; ObjectProperty is assigned between them.

More complex example: Input A and B have to go into a process, while Input C and D are alternatives for A and B. The Inputs have to go as groups in the process. This equals: A AND B OR C AND D. The Dependency Operator is used between A and B as well as between C and D.

Furthermore, the Operator can be used to express dependencies between In- and Outputs. If A and B are alternative Inputs that result in the Ouputs C for A or D for B then this equals: A AND C or D AND B. The ObjectProperty can be used between both, In- and/or Outputs.</rdfs:comment>
    </owl:ObjectProperty>
    


    <!-- http://www.hsu-ifa.de/ontologies/VDI3682#downFlow -->

    <owl:ObjectProperty rdf:about="http://www.hsu-ifa.de/ontologies/VDI3682#downFlow">
        <rdfs:subPropertyOf rdf:resource="http://www.hsu-ifa.de/ontologies/VDI3682#flow"/>
        <rdfs:comment>a downflow occurs whenever one tries to follow an entity down the value stream to the end of production</rdfs:comment>
    </owl:ObjectProperty>
    


    <!-- http://www.hsu-ifa.de/ontologies/VDI3682#flow -->

    <owl:ObjectProperty rdf:about="http://www.hsu-ifa.de/ontologies/VDI3682#flow">
        <rdfs:comment>most generic concept for flows taken from VDI3682 and refined by semantics that is used in graphical notation</rdfs:comment>
    </owl:ObjectProperty>
    


    <!-- http://www.hsu-ifa.de/ontologies/VDI3682#hasAlternativeInput -->

    <owl:ObjectProperty rdf:about="http://www.hsu-ifa.de/ontologies/VDI3682#hasAlternativeInput">
        <rdfs:subPropertyOf rdf:resource="http://www.hsu-ifa.de/ontologies/VDI3682#hasInput"/>
    </owl:ObjectProperty>
    


    <!-- http://www.hsu-ifa.de/ontologies/VDI3682#hasAlternativeOutput -->

    <owl:ObjectProperty rdf:about="http://www.hsu-ifa.de/ontologies/VDI3682#hasAlternativeOutput">
        <rdfs:subPropertyOf rdf:resource="http://www.hsu-ifa.de/ontologies/VDI3682#hasOutput"/>
    </owl:ObjectProperty>
    


    <!-- http://www.hsu-ifa.de/ontologies/VDI3682#hasChild -->

    <owl:ObjectProperty rdf:about="http://www.hsu-ifa.de/ontologies/VDI3682#hasChild">
        <rdfs:subPropertyOf rdf:resource="http://www.w3.org/2002/07/owl#topObjectProperty"/>
        <owl:inverseOf rdf:resource="http://www.hsu-ifa.de/ontologies/VDI3682#hasParent"/>
        <rdf:type rdf:resource="http://www.w3.org/2002/07/owl#TransitiveProperty"/>
        <rdfs:comment>as the formalized process description does not classifiy processes, products or other entities, this relation can be used to indicate inheritance</rdfs:comment>
    </owl:ObjectProperty>
    


    <!-- http://www.hsu-ifa.de/ontologies/VDI3682#hasInput -->

    <owl:ObjectProperty rdf:about="http://www.hsu-ifa.de/ontologies/VDI3682#hasInput">
        <rdfs:subPropertyOf rdf:resource="http://www.hsu-ifa.de/ontologies/VDI3682#upFlow"/>
        <owl:inverseOf rdf:resource="http://www.hsu-ifa.de/ontologies/VDI3682#isInputFor"/>
        <rdfs:domain rdf:resource="http://www.hsu-ifa.de/ontologies/VDI3682#Process"/>
        <rdfs:range>
            <owl:Class>
                <owl:unionOf rdf:parseType="Collection">
                    <rdf:Description rdf:about="http://www.hsu-ifa.de/ontologies/VDI3682#Energy"/>
                    <rdf:Description rdf:about="http://www.hsu-ifa.de/ontologies/VDI3682#Information"/>
                    <rdf:Description rdf:about="http://www.hsu-ifa.de/ontologies/VDI3682#Product"/>
                </owl:unionOf>
            </owl:Class>
        </rdfs:range>
        <rdfs:comment>ObjectProperty that is used to link a ProcessOperator with an Input, i.e. Energy or Information or Product.</rdfs:comment>
    </owl:ObjectProperty>
    


    <!-- http://www.hsu-ifa.de/ontologies/VDI3682#hasOutput -->

    <owl:ObjectProperty rdf:about="http://www.hsu-ifa.de/ontologies/VDI3682#hasOutput">
        <rdfs:subPropertyOf rdf:resource="http://www.hsu-ifa.de/ontologies/VDI3682#downFlow"/>
        <owl:inverseOf rdf:resource="http://www.hsu-ifa.de/ontologies/VDI3682#isOutputOf"/>
        <rdfs:domain rdf:resource="http://www.hsu-ifa.de/ontologies/VDI3682#Process"/>
        <rdfs:range>
            <owl:Class>
                <owl:unionOf rdf:parseType="Collection">
                    <rdf:Description rdf:about="http://www.hsu-ifa.de/ontologies/VDI3682#Energy"/>
                    <rdf:Description rdf:about="http://www.hsu-ifa.de/ontologies/VDI3682#Information"/>
                    <rdf:Description rdf:about="http://www.hsu-ifa.de/ontologies/VDI3682#Product"/>
                </owl:unionOf>
            </owl:Class>
        </rdfs:range>
        <rdfs:comment>ObjectProperty that is used to link a ProcessOperator with an Output, i.e. Energy or Information or Product.</rdfs:comment>
    </owl:ObjectProperty>
    


    <!-- http://www.hsu-ifa.de/ontologies/VDI3682#hasParallelInput -->

    <owl:ObjectProperty rdf:about="http://www.hsu-ifa.de/ontologies/VDI3682#hasParallelInput">
        <rdfs:subPropertyOf rdf:resource="http://www.hsu-ifa.de/ontologies/VDI3682#hasInput"/>
    </owl:ObjectProperty>
    


    <!-- http://www.hsu-ifa.de/ontologies/VDI3682#hasParallelOutput -->

    <owl:ObjectProperty rdf:about="http://www.hsu-ifa.de/ontologies/VDI3682#hasParallelOutput">
        <rdfs:subPropertyOf rdf:resource="http://www.hsu-ifa.de/ontologies/VDI3682#hasOutput"/>
    </owl:ObjectProperty>
    


    <!-- http://www.hsu-ifa.de/ontologies/VDI3682#hasParent -->

    <owl:ObjectProperty rdf:about="http://www.hsu-ifa.de/ontologies/VDI3682#hasParent">
        <rdf:type rdf:resource="http://www.w3.org/2002/07/owl#TransitiveProperty"/>
        <rdfs:comment>as the formalized process description does not classifiy processes, products or other entities, this relation can be used to indicate inheritance</rdfs:comment>
    </owl:ObjectProperty>
    


    <!-- http://www.hsu-ifa.de/ontologies/VDI3682#hasPredecessor -->

    <owl:ObjectProperty rdf:about="http://www.hsu-ifa.de/ontologies/VDI3682#hasPredecessor">
        <owl:inverseOf rdf:resource="http://www.hsu-ifa.de/ontologies/VDI3682#hasSuccessor"/>
        <rdf:type rdf:resource="http://www.w3.org/2002/07/owl#TransitiveProperty"/>
        <owl:propertyChainAxiom rdf:parseType="Collection">
            <rdf:Description rdf:about="http://www.hsu-ifa.de/ontologies/VDI3682#upFlow"/>
            <rdf:Description rdf:about="http://www.hsu-ifa.de/ontologies/VDI3682#upFlow"/>
        </owl:propertyChainAxiom>
        <rdfs:comment>an object property that is used to infer a predecessing relationship between entities</rdfs:comment>
    </owl:ObjectProperty>
    


    <!-- http://www.hsu-ifa.de/ontologies/VDI3682#hasState -->

    <owl:ObjectProperty rdf:about="http://www.hsu-ifa.de/ontologies/VDI3682#hasState">
        <rdfs:domain>
            <owl:Class>
                <owl:unionOf rdf:parseType="Collection">
                    <rdf:Description rdf:about="http://www.hsu-ifa.de/ontologies/VDI3682#Energy"/>
                    <rdf:Description rdf:about="http://www.hsu-ifa.de/ontologies/VDI3682#Information"/>
                    <rdf:Description rdf:about="http://www.hsu-ifa.de/ontologies/VDI3682#Product"/>
                </owl:unionOf>
            </owl:Class>
        </rdfs:domain>
        <rdfs:range rdf:resource="http://www.hsu-ifa.de/ontologies/VDI3682#State"/>
        <rdfs:comment>ObjectProperty that is used to describe the state of a process via the state of products, energies and information.</rdfs:comment>
    </owl:ObjectProperty>
    


    <!-- http://www.hsu-ifa.de/ontologies/VDI3682#hasSubProcess -->

    <owl:ObjectProperty rdf:about="http://www.hsu-ifa.de/ontologies/VDI3682#hasSubProcess">
        <owl:inverseOf rdf:resource="http://www.hsu-ifa.de/ontologies/VDI3682#hasUpperProcess"/>
        <rdf:type rdf:resource="http://www.w3.org/2002/07/owl#AsymmetricProperty"/>
        <rdf:type rdf:resource="http://www.w3.org/2002/07/owl#IrreflexiveProperty"/>
        <rdfs:domain rdf:resource="http://www.hsu-ifa.de/ontologies/VDI3682#Process"/>
        <rdfs:range rdf:resource="http://www.hsu-ifa.de/ontologies/VDI3682#Process"/>
        <rdfs:comment>ObjectProperty that is used for decomposition of process operators.</rdfs:comment>
    </owl:ObjectProperty>
    


    <!-- http://www.hsu-ifa.de/ontologies/VDI3682#hasSuccessor -->

    <owl:ObjectProperty rdf:about="http://www.hsu-ifa.de/ontologies/VDI3682#hasSuccessor">
        <rdf:type rdf:resource="http://www.w3.org/2002/07/owl#TransitiveProperty"/>
        <owl:propertyChainAxiom rdf:parseType="Collection">
            <rdf:Description rdf:about="http://www.hsu-ifa.de/ontologies/VDI3682#downFlow"/>
            <rdf:Description rdf:about="http://www.hsu-ifa.de/ontologies/VDI3682#downFlow"/>
        </owl:propertyChainAxiom>
        <rdfs:comment>an object property that is used to infer a successing relationshipt between entities</rdfs:comment>
    </owl:ObjectProperty>
    


    <!-- http://www.hsu-ifa.de/ontologies/VDI3682#hasUpperProcess -->

    <owl:ObjectProperty rdf:about="http://www.hsu-ifa.de/ontologies/VDI3682#hasUpperProcess">
        <rdf:type rdf:resource="http://www.w3.org/2002/07/owl#AsymmetricProperty"/>
        <rdf:type rdf:resource="http://www.w3.org/2002/07/owl#IrreflexiveProperty"/>
        <rdfs:domain rdf:resource="http://www.hsu-ifa.de/ontologies/VDI3682#Process"/>
        <rdfs:range rdf:resource="http://www.hsu-ifa.de/ontologies/VDI3682#Process"/>
    </owl:ObjectProperty>
    


    <!-- http://www.hsu-ifa.de/ontologies/VDI3682#isAlternativeInputFor -->

    <owl:ObjectProperty rdf:about="http://www.hsu-ifa.de/ontologies/VDI3682#isAlternativeInputFor">
        <rdfs:subPropertyOf rdf:resource="http://www.hsu-ifa.de/ontologies/VDI3682#isInputFor"/>
    </owl:ObjectProperty>
    


    <!-- http://www.hsu-ifa.de/ontologies/VDI3682#isAlternativeOutputOf -->

    <owl:ObjectProperty rdf:about="http://www.hsu-ifa.de/ontologies/VDI3682#isAlternativeOutputOf">
        <rdfs:subPropertyOf rdf:resource="http://www.hsu-ifa.de/ontologies/VDI3682#isOutputOf"/>
    </owl:ObjectProperty>
    


    <!-- http://www.hsu-ifa.de/ontologies/VDI3682#isInputFor -->

    <owl:ObjectProperty rdf:about="http://www.hsu-ifa.de/ontologies/VDI3682#isInputFor">
        <rdfs:subPropertyOf rdf:resource="http://www.hsu-ifa.de/ontologies/VDI3682#downFlow"/>
        <rdfs:domain>
            <owl:Class>
                <owl:unionOf rdf:parseType="Collection">
                    <rdf:Description rdf:about="http://www.hsu-ifa.de/ontologies/VDI3682#Energy"/>
                    <rdf:Description rdf:about="http://www.hsu-ifa.de/ontologies/VDI3682#Information"/>
                    <rdf:Description rdf:about="http://www.hsu-ifa.de/ontologies/VDI3682#Product"/>
                </owl:unionOf>
            </owl:Class>
        </rdfs:domain>
        <rdfs:range rdf:resource="http://www.hsu-ifa.de/ontologies/VDI3682#Process"/>
        <rdfs:comment>the inverse of &quot;hasIntput&quot;</rdfs:comment>
    </owl:ObjectProperty>
    


    <!-- http://www.hsu-ifa.de/ontologies/VDI3682#isOnSystemBorder -->

    <owl:ObjectProperty rdf:about="http://www.hsu-ifa.de/ontologies/VDI3682#isOnSystemBorder">
        <rdfs:domain>
            <owl:Class>
                <owl:unionOf rdf:parseType="Collection">
                    <rdf:Description rdf:about="http://www.hsu-ifa.de/ontologies/VDI3682#Energy"/>
                    <rdf:Description rdf:about="http://www.hsu-ifa.de/ontologies/VDI3682#Information"/>
                    <rdf:Description rdf:about="http://www.hsu-ifa.de/ontologies/VDI3682#Product"/>
                </owl:unionOf>
            </owl:Class>
        </rdfs:domain>
        <rdfs:range rdf:resource="http://www.hsu-ifa.de/ontologies/VDI3682#SystemBorder"/>
        <rdfs:comment>Objectproperty that is used to assign an In- or Output to be coming from outside of the system boarder.</rdfs:comment>
    </owl:ObjectProperty>
    


    <!-- http://www.hsu-ifa.de/ontologies/VDI3682#isOutputOf -->

    <owl:ObjectProperty rdf:about="http://www.hsu-ifa.de/ontologies/VDI3682#isOutputOf">
        <rdfs:subPropertyOf rdf:resource="http://www.hsu-ifa.de/ontologies/VDI3682#upFlow"/>
        <rdfs:domain>
            <owl:Class>
                <owl:unionOf rdf:parseType="Collection">
                    <rdf:Description rdf:about="http://www.hsu-ifa.de/ontologies/VDI3682#Energy"/>
                    <rdf:Description rdf:about="http://www.hsu-ifa.de/ontologies/VDI3682#Information"/>
                    <rdf:Description rdf:about="http://www.hsu-ifa.de/ontologies/VDI3682#Product"/>
                </owl:unionOf>
            </owl:Class>
        </rdfs:domain>
        <rdfs:range rdf:resource="http://www.hsu-ifa.de/ontologies/VDI3682#Process"/>
        <rdfs:comment>the inverse of &quot;hasOutput&quot;</rdfs:comment>
    </owl:ObjectProperty>
    


    <!-- http://www.hsu-ifa.de/ontologies/VDI3682#isParallelInputFor -->

    <owl:ObjectProperty rdf:about="http://www.hsu-ifa.de/ontologies/VDI3682#isParallelInputFor">
        <rdfs:subPropertyOf rdf:resource="http://www.hsu-ifa.de/ontologies/VDI3682#isInputFor"/>
    </owl:ObjectProperty>
    


    <!-- http://www.hsu-ifa.de/ontologies/VDI3682#isParallelOutputOf -->

    <owl:ObjectProperty rdf:about="http://www.hsu-ifa.de/ontologies/VDI3682#isParallelOutputOf">
        <rdfs:subPropertyOf rdf:resource="http://www.hsu-ifa.de/ontologies/VDI3682#isOutputOf"/>
    </owl:ObjectProperty>
    


    <!-- http://www.hsu-ifa.de/ontologies/VDI3682#isWithinSystemBorder -->

    <owl:ObjectProperty rdf:about="http://www.hsu-ifa.de/ontologies/VDI3682#isWithinSystemBorder">
        <rdfs:domain>
            <owl:Class>
                <owl:unionOf rdf:parseType="Collection">
                    <rdf:Description rdf:about="http://www.hsu-ifa.de/ontologies/VDI3682#Energy"/>
                    <rdf:Description rdf:about="http://www.hsu-ifa.de/ontologies/VDI3682#Information"/>
                    <rdf:Description rdf:about="http://www.hsu-ifa.de/ontologies/VDI3682#Process"/>
                    <rdf:Description rdf:about="http://www.hsu-ifa.de/ontologies/VDI3682#Product"/>
                </owl:unionOf>
            </owl:Class>
        </rdfs:domain>
        <rdfs:range rdf:resource="http://www.hsu-ifa.de/ontologies/VDI3682#SystemBorder"/>
        <rdfs:comment>ObjectProperty that is used to indicate that a process operator is within a certain system boarder.</rdfs:comment>
    </owl:ObjectProperty>
    


    <!-- http://www.hsu-ifa.de/ontologies/VDI3682#upFlow -->

    <owl:ObjectProperty rdf:about="http://www.hsu-ifa.de/ontologies/VDI3682#upFlow">
        <rdfs:subPropertyOf rdf:resource="http://www.hsu-ifa.de/ontologies/VDI3682#flow"/>
        <rdfs:comment>an upflow occurs whenever one tries to trace from a starting point up the value stream to the beginning of production</rdfs:comment>
    </owl:ObjectProperty>
    


    <!-- 
    ///////////////////////////////////////////////////////////////////////////////////////
    //
    // Data properties
    //
    ///////////////////////////////////////////////////////////////////////////////////////
     -->

    


    <!-- http://www.hsu-ifa.de/ontologies/VDI3682#longName -->

    <owl:DatatypeProperty rdf:about="http://www.hsu-ifa.de/ontologies/VDI3682#longName">
        <rdf:type rdf:resource="http://www.w3.org/2002/07/owl#FunctionalProperty"/>
        <rdfs:comment>A property that is used to give a long name to an individual.</rdfs:comment>
    </owl:DatatypeProperty>
    


    <!-- http://www.hsu-ifa.de/ontologies/VDI3682#shortName -->

    <owl:DatatypeProperty rdf:about="http://www.hsu-ifa.de/ontologies/VDI3682#shortName">
        <rdf:type rdf:resource="http://www.w3.org/2002/07/owl#FunctionalProperty"/>
        <rdfs:comment>A property that is used to give a short name to an individual.</rdfs:comment>
    </owl:DatatypeProperty>
    


    <!-- 
    ///////////////////////////////////////////////////////////////////////////////////////
    //
    // Classes
    //
    ///////////////////////////////////////////////////////////////////////////////////////
     -->

    


    <!-- http://www.hsu-ifa.de/ontologies/VDI3682#Energy -->

    <owl:Class rdf:about="http://www.hsu-ifa.de/ontologies/VDI3682#Energy">
        <rdfs:comment>Energy is requiered by the process operator to fullfill the process. Energy is Input and Output of a process. Energy can be any kind of energy, exp.: electricity, heat,...</rdfs:comment>
    </owl:Class>
    


    <!-- http://www.hsu-ifa.de/ontologies/VDI3682#Information -->

    <owl:Class rdf:about="http://www.hsu-ifa.de/ontologies/VDI3682#Information">
        <rdfs:comment>Information input for a process operator can be any kind of information required to fullfill the process. Information output can be any kind of information created by the process.
[VDI 3682-1]</rdfs:comment>
    </owl:Class>
    


    <!-- http://www.hsu-ifa.de/ontologies/VDI3682#Process -->

    <owl:Class rdf:about="http://www.hsu-ifa.de/ontologies/VDI3682#Process">
        <rdfs:subClassOf>
            <owl:Restriction>
                <owl:onProperty rdf:resource="http://www.hsu-ifa.de/ontologies/VDI3682#hasInput"/>
                <owl:minQualifiedCardinality rdf:datatype="http://www.w3.org/2001/XMLSchema#nonNegativeInteger">1</owl:minQualifiedCardinality>
                <owl:onClass>
                    <owl:Class>
                        <owl:unionOf rdf:parseType="Collection">
                            <rdf:Description rdf:about="http://www.hsu-ifa.de/ontologies/VDI3682#Energy"/>
                            <rdf:Description rdf:about="http://www.hsu-ifa.de/ontologies/VDI3682#Information"/>
                            <rdf:Description rdf:about="http://www.hsu-ifa.de/ontologies/VDI3682#Product"/>
                        </owl:unionOf>
                    </owl:Class>
                </owl:onClass>
            </owl:Restriction>
        </rdfs:subClassOf>
        <rdfs:subClassOf>
            <owl:Restriction>
                <owl:onProperty rdf:resource="http://www.hsu-ifa.de/ontologies/VDI3682#hasOutput"/>
                <owl:minQualifiedCardinality rdf:datatype="http://www.w3.org/2001/XMLSchema#nonNegativeInteger">1</owl:minQualifiedCardinality>
                <owl:onClass>
                    <owl:Class>
                        <owl:unionOf rdf:parseType="Collection">
                            <rdf:Description rdf:about="http://www.hsu-ifa.de/ontologies/VDI3682#Energy"/>
                            <rdf:Description rdf:about="http://www.hsu-ifa.de/ontologies/VDI3682#Information"/>
                            <rdf:Description rdf:about="http://www.hsu-ifa.de/ontologies/VDI3682#Product"/>
                        </owl:unionOf>
                    </owl:Class>
                </owl:onClass>
            </owl:Restriction>
        </rdfs:subClassOf>
        <rdfs:comment>A process describes the desired behavior of a process operator, by means of a solution neutral description of inputs and outputs. Products,energies  and information are converted into new products,energies  and information by a process operator. The process operator implements this conversion with the help of technical resources.

[VDI3682]</rdfs:comment>
    </owl:Class>
    


    <!-- http://www.hsu-ifa.de/ontologies/VDI3682#Product -->

    <owl:Class rdf:about="http://www.hsu-ifa.de/ontologies/VDI3682#Product"/>
    


    <!-- http://www.hsu-ifa.de/ontologies/VDI3682#State -->

    <owl:Class rdf:about="http://www.hsu-ifa.de/ontologies/VDI3682#State">
        <rdfs:comment>A State describes the actual state of a Product/Energy/Information. Exp.: status ante operationem and status post operationem.
[VDI3682-1]</rdfs:comment>
    </owl:Class>
    


    <!-- http://www.hsu-ifa.de/ontologies/VDI3682#SystemBorder -->

    <owl:Class rdf:about="http://www.hsu-ifa.de/ontologies/VDI3682#SystemBorder">
        <rdfs:comment>The system boundary determines the observation horizon of the process. In a broader sense, this can also be seen as the balance limit for incoming products/energy/information and outgoing products/energy/information.
[VDI 3682-1]</rdfs:comment>
    </owl:Class>
    


    <!-- http://www.hsu-ifa.de/ontologies/VDI3682#TechnicalResource -->

    <owl:Class rdf:about="http://www.hsu-ifa.de/ontologies/VDI3682#TechnicalResource">
        <rdfs:comment>The technical resource is able to implement certain processes and is an abstract description of a system.
[VDI 3682-1]</rdfs:comment>
    </owl:Class>
    


    <!-- 
    ///////////////////////////////////////////////////////////////////////////////////////
    //
    // General axioms
    //
    ///////////////////////////////////////////////////////////////////////////////////////
     -->

    <rdf:Description>
        <rdf:type rdf:resource="http://www.w3.org/2002/07/owl#AllDisjointClasses"/>
        <owl:members rdf:parseType="Collection">
            <rdf:Description rdf:about="http://www.hsu-ifa.de/ontologies/VDI3682#Energy"/>
            <rdf:Description rdf:about="http://www.hsu-ifa.de/ontologies/VDI3682#Information"/>
            <rdf:Description rdf:about="http://www.hsu-ifa.de/ontologies/VDI3682#Product"/>
            <rdf:Description rdf:about="http://www.hsu-ifa.de/ontologies/VDI3682#State"/>
            <rdf:Description rdf:about="http://www.hsu-ifa.de/ontologies/VDI3682#SystemBorder"/>
            <rdf:Description rdf:about="http://www.hsu-ifa.de/ontologies/VDI3682#TechnicalResource"/>
        </owl:members>
    </rdf:Description>
</rdf:RDF>



<!-- Generated by the OWL API (version 4.2.8.20170104-2310) https://github.com/owlcs/owlapi -->

